Proof of alloc_disjoint using ctrees. Had to unset universe checking to import FoldStateT.

src/rocq/Utils/CTreeMemExample.v
@@ -1,7 +1,7 @@
-From Paco Require Import paco.
+Unset Universe Checking.
 
 From CTree Require Import
-  CTree CTreeDefinitions Eq Fold.
+  CTree CTreeDefinitions Eq Fold FoldStateT.
 
 From Vellvm.Utils Require Import Tactics.
 
@@ -361,6 +361,7 @@ destruct (IM.mem (elt:=nat) (next_key m) m) eqn:MEM; auto.
 apply IM.mem_2 in MEM.
 apply next_key_correct in MEM.
 lia.
+
 Abort.
 
 (* 
@@ -777,357 +778,13 @@ intros s.
 apply mstuck.
 Defined.
 
-#[global] Instance MonadBrState {B S M} `{HM : Monad M} `{MB : MonadBr B M} `{FB : Functor B}: MonadBr B (stateT S M).
+#[global] Instance MonadBrState {B S M} `{HM : Monad M} `{MB : MonadBr B M} : MonadBr B (stateT S M).
 red.
 intros X b s.
-apply mbr.
-eapply fmap in b.
-apply b.
-intros x.
-apply (s, x).
+apply mbr in b.
+eapply fmap; cycle 1; eauto.
 Defined.
 
-Definition interp_state {E B M S}
-  {FB : Functor B}
-  {FM : Functor M} {MM : Monad M}
-  {IM : MonadIter M}
-  {MSTUCK : MonadStuck M}
-  {MSTEP : MonadStep M}
-  {MBR : MonadBr B M}
-  (h : E ~> stateT S M) :
-  ctree E B ~> stateT S M := interp h.
-
-Arguments interp_state {E B M S FB FM MM IM MSTUCK MSTEP MBR} h [T].
-
-(* Definition _interp_state {E F C D S R} *)
-(*            (f : E ~> stateT S (ctree F D)) (ot : ctreeF E C R _) *)
-(*   : stateT S (ctree F D) R := *)
-(*   fun s => *)
-(*     match ot with *)
-(*     | RetF r => Ret (s, r) *)
-(*     | StuckF => Stuck *)
-(*     | StepF t => StepF  *)
-(*     | GuardF t => _ *)
-(*     | VisF X e k => _ *)
-(*     | BrF X c k => _ *)
-(*     end. *)
-(*   match ot with *)
-(*   | RetF r => Ret (s, r) *)
-(*   | TauF t => Tau (interp_state f t s) *)
-(*   | VisF e k => f _ e s >>= (fun sx => Tau (interp_state f (k (snd sx)) (fst sx))) *)
-(*   end. *)
-
-(* Lemma unfold_interp_state {E F S R} (h : E ~> Monads.stateT S (itree F)) *)
-(*       (t : itree E R) s : *)
-(*     eq_itree eq *)
-(*       (interp_state h t s) *)
-(*       (_interp_state h (observe t) s). *)
-(* Proof. *)
-(*   unfold interp_state, interp, Basics.iter, MonadIter_stateT0, Basics.iter, MonadIter_itree; cbn. *)
-(*   rewrite unfold_iter; cbn. *)
-(*   destruct observe; cbn. *)
-(*   - rewrite 2 bind_ret_l. reflexivity. *)
-(*   - rewrite 2 bind_ret_l. *)
-(*     reflexivity. *)
-(*   - rewrite bind_map, bind_bind; cbn. setoid_rewrite bind_ret_l. *)
-(*     apply eqit_bind; reflexivity. *)
-(* Qed. *)
-
-(* #[global] *)
-(* Instance eq_itree_interp_state {E F S R} (h : E ~> Monads.stateT S (itree F)) : *)
-(*   Proper (eq_itree eq ==> eq ==> eq_itree eq) *)
-(*          (@interp_state _ _ _ _ _ _ h R). *)
-(* Proof. *)
-(*   revert_until R. *)
-(*   ginit. pcofix CIH. intros h x y H0 x2 _ []. *)
-(*   rewrite !unfold_interp_state. *)
-(*   punfold H0; repeat red in H0. *)
-(*   destruct H0; subst; pclearbot; try discriminate; cbn. *)
-(*   - gstep; constructor; auto. *)
-(*   - gstep; constructor; auto with paco. *)
-(*   - guclo eqit_clo_bind. econstructor. *)
-(*     + reflexivity. *)
-(*     + intros [] _ []. gstep; constructor; auto with paco itree. *)
-(* Qed. *)
-
-(* Lemma interp_state_ret {E F : Type -> Type} {R S : Type} *)
-(*       (f : forall T, E T -> S -> itree F (S * T)%type) *)
-(*       (s : S) (r : R) : *)
-(*   (interp_state f (Ret r) s) ≅ (Ret (s, r)). *)
-(* Proof. *)
-(*   rewrite itree_eta. reflexivity. *)
-(* Qed. *)
-
-(* Lemma interp_state_vis {E F : Type -> Type} {S T U : Type} *)
-(*       (e : E T) (k : T -> itree E U) (h : E ~> Monads.stateT S (itree F)) (s : S) *)
-(*   : interp_state h (Vis e k) s *)
-(*   ≅ h T e s >>= fun sx => Tau (interp_state h (k (snd sx)) (fst sx)). *)
-(* Proof. *)
-(*   rewrite unfold_interp_state; reflexivity. *)
-(* Qed. *)
-
-(* Lemma interp_state_tau {E F : Type -> Type} S {T : Type} *)
-(*       (t : itree E T) (h : E ~> Monads.stateT S (itree F)) (s : S) *)
-(*   : interp_state h (Tau t) s ≅ Tau (interp_state h t s). *)
-(* Proof. *)
-(*   rewrite unfold_interp_state; reflexivity. *)
-(* Qed. *)
-
-(* Lemma interp_state_trigger_eqit {E F : Type -> Type} {R S : Type} *)
-(*       (e : E R) (f : E ~> Monads.stateT S (itree F)) (s : S) *)
-(*   : (interp_state f (ITree.trigger e) s) ≅ (f _ e s >>= fun x => Tau (Ret x)). *)
-(* Proof. *)
-(*   unfold ITree.trigger. rewrite interp_state_vis. *)
-(*   eapply eqit_bind; try reflexivity. *)
-(*   intros []. rewrite interp_state_ret. reflexivity. *)
-(* Qed. *)
-
-(* Lemma interp_state_trigger {E F : Type -> Type} {R S : Type} *)
-(*       (e : E R) (f : E ~> Monads.stateT S (itree F)) (s : S) *)
-(*   : interp_state f (ITree.trigger e) s ≈ f _ e s. *)
-(* Proof. *)
-(*   unfold ITree.trigger. rewrite interp_state_vis. *)
-(*   match goal with *)
-(*     |- ?y ≈ ?x => remember y; rewrite <- (bind_ret_r x); subst *)
-(*   end. *)
-(*   eapply eqit_bind; try reflexivity. *)
-(*   intros []; rewrite interp_state_ret,tau_eutt. *)
-(*   reflexivity. *)
-(* Qed. *)
-
-(* Lemma interp_state_bind {E F : Type -> Type} {A B S : Type} *)
-(*       (f : forall T, E T -> S -> itree F (S * T)%type) *)
-(*       (t : itree E A) (k : A -> itree E B) *)
-(*       (s : S) : *)
-(*   (interp_state f (t >>= k) s) *)
-(*     ≅ *)
-(*   (interp_state f t s >>= fun st => interp_state f (k (snd st)) (fst st)). *)
-(* Proof. *)
-(*   revert t k s. *)
-(*   ginit. pcofix CIH. *)
-(*   intros t k s. *)
-(*   rewrite unfold_bind. *)
-(*   rewrite (unfold_interp_state f t). *)
-(*   destruct (observe t). *)
-(*   - cbn. rewrite !bind_ret_l. cbn. *)
-(*     apply reflexivity. *)
-(*   - cbn. rewrite !bind_tau, interp_state_tau. *)
-(*     gstep. econstructor. gbase. apply CIH. *)
-(*   - cbn. rewrite interp_state_vis, bind_bind. *)
-(*     guclo eqit_clo_bind. econstructor. *)
-(*     + reflexivity. *)
-(*     + intros u2 ? []. *)
-(*       rewrite bind_tau. *)
-(*       gstep; constructor. *)
-(*       ITree.fold_subst. *)
-(*       auto with paco. *)
-(* Qed. *)
-
-(* #[global] *)
-(* Instance eutt_interp_state {E F: Type -> Type} {S : Type} *)
-(*          (h : E ~> Monads.stateT S (itree F)) R RR : *)
-(*   Proper (eutt RR ==> eq ==> eutt (prod_rel eq RR)) (@interp_state E (itree F) S _ _ _ h R). *)
-(* Proof. *)
-(*   repeat intro. subst. revert_until RR. *)
-(*   einit. ecofix CIH. intros. *)
-
-(*   rewrite !unfold_interp_state. punfold H0. red in H0. *)
-(*   induction H0; intros; subst; simpl; pclearbot. *)
-(*   - eret. *)
-(*   - etau. *)
-(*   - ebind. econstructor; [reflexivity|]. *)
-(*     intros; subst. *)
-(*     etau. ebase. *)
-(*   - rewrite tau_euttge, unfold_interp_state; eauto. *)
-(*   - rewrite tau_euttge, unfold_interp_state; eauto. *)
-(* Qed. *)
-
-(* #[global] *)
-(* Instance eutt_interp_state_eq {E F: Type -> Type} {S : Type} *)
-(*          (h : E ~> Monads.stateT S (itree F)) R : *)
-(*   Proper (eutt eq ==> eq ==> eutt eq) (@interp_state E (itree F) S _ _ _ h R). *)
-(* Proof. *)
-(*   repeat intro. subst. revert_until R. *)
-(*   einit. ecofix CIH. intros. *)
-
-(*   rewrite !unfold_interp_state. punfold H0. red in H0. *)
-(*   induction H0; intros; subst; simpl; pclearbot. *)
-(*   - eret. *)
-(*   - etau. *)
-(*   - ebind. econstructor; [reflexivity|]. *)
-(*     intros; subst. *)
-(*     etau. ebase. *)
-(*   - rewrite tau_euttge, unfold_interp_state; eauto. *)
-(*   - rewrite tau_euttge, unfold_interp_state; eauto. *)
-(* Qed. *)
-
-
-(* Lemma eutt_interp_state_aloop {E F S I I' A A'} *)
-(*       (RA : A -> A' -> Prop) (RI : I -> I' -> Prop) *)
-(*       (RS : S -> S -> Prop) *)
-(*       (h : E ~> Monads.stateT S (itree F)) *)
-(*       (t1 : I -> itree E (I + A)) *)
-(*       (t2 : I' -> itree E (I' + A')): *)
-(*   (forall i i' s1 s2, RS s1 s2 -> RI i i' -> *)
-(*      eutt (prod_rel RS (sum_rel RI RA)) *)
-(*                      (interp_state h (t1 i) s1) *)
-(*                      (interp_state h (t2 i') s2)) -> *)
-(*   (forall i i' s1 s2, RS s1 s2 -> RI i i' -> *)
-(*      eutt (fun a b => RS (fst a) (fst b) /\ RA (snd a) (snd b)) *)
-(*           (interp_state h (ITree.iter t1 i) s1) *)
-(*           (interp_state h (ITree.iter t2 i') s2)). *)
-(* Proof. *)
-(*   intro Ht. *)
-(*   einit. ecofix CIH. intros. *)
-(*   rewrite 2 unfold_iter. *)
-(*   rewrite 2 interp_state_bind. *)
-(*   ebind; econstructor. *)
-(*   - eapply Ht; auto. *)
-(*   - intros [s1' i1'] [s2' i2'] [? []]; cbn. *)
-(*     + rewrite 2 interp_state_tau. auto with paco. *)
-(*     + rewrite 2 interp_state_ret. auto with paco. *)
-(* Qed. *)
-
-(* Lemma eutt_interp_state_iter {E F S A A' B B'} *)
-(*       (RA : A -> A' -> Prop) (RB : B -> B' -> Prop) *)
-(*       (RS : S -> S -> Prop) *)
-(*       (h : E ~> Monads.stateT S (itree F)) *)
-(*       (t1 : A -> itree E (A + B)) *)
-(*       (t2 : A' -> itree E (A' + B')) : *)
-(*   (forall ca ca' s1 s2, RS s1 s2 -> *)
-(*                         RA ca ca' -> *)
-(*      eutt (prod_rel RS (sum_rel RA RB)) *)
-(*           (interp_state h (t1 ca) s1) *)
-(*           (interp_state h (t2 ca') s2)) -> *)
-(*   (forall a a' s1 s2, RS s1 s2 -> RA a a' -> *)
-(*      eutt (fun a b => RS (fst a) (fst b) /\ RB (snd a) (snd b)) *)
-(*           (interp_state h (iter (C := ktree _) t1 a) s1) *)
-(*           (interp_state h (iter (C := ktree _) t2 a') s2)). *)
-(* Proof. *)
-(*   apply eutt_interp_state_aloop. *)
-(* Qed. *)
-
-(* Lemma eutt_eq_interp_state_iter {E F S} (f: E ~> stateT S (itree F)) {I A} *)
-(*     (t : I -> itree E (I + A)): *)
-(*   forall i s, interp_state f (ITree.iter t i) s ≈ *)
-(*     Basics.iter (fun i => interp_state f (t i)) i s. *)
-(* Proof. *)
-(*   unfold Basics.iter, MonadIter_stateT0, Basics.iter, MonadIter_itree in *; cbn. *)
-(*   ginit. gcofix CIH; intros i s. *)
-(*   rewrite 2 unfold_iter; cbn. *)
-(*   rewrite !bind_bind. *)
-(*   setoid_rewrite bind_ret_l. *)
-(*   rewrite interp_state_bind. *)
-(*   guclo eqit_clo_bind; econstructor; eauto. reflexivity. *)
-(*   intros [s' []] _ []; cbn. *)
-(*   - rewrite interp_state_tau. *)
-(*     gstep; constructor. *)
-(*     auto with paco. *)
-(*   - rewrite interp_state_ret; apply reflexivity. *)
-(* Qed. *)
-
-(* Lemma eutt_interp_state_loop {E F S A B C} (RS : S -> S -> Prop) *)
-(*       (h : E ~> Monads.stateT S (itree F)) *)
-(*       (t1 t2 : C + A -> itree E (C + B)) : *)
-(*   (forall ca s1 s2, RS s1 s2 -> *)
-(*      eutt (fun a b => RS (fst a) (fst b) /\ snd a = snd b) *)
-(*           (interp_state h (t1 ca) s1) *)
-(*           (interp_state h (t2 ca) s2)) -> *)
-(*   (forall a s1 s2, RS s1 s2 -> *)
-(*      eutt (fun a b => RS (fst a) (fst b) /\ snd a = snd b) *)
-(*           (interp_state h (loop (C := ktree E) t1 a) s1) *)
-(*           (interp_state h (loop (C := ktree E) t2 a) s2)). *)
-(* Proof. *)
-(*   intros. *)
-(*   unfold loop, bimap, Bimap_Coproduct, case_, Case_Kleisli, Function.case_sum, id_, Id_Kleisli, cat, Cat_Kleisli, inr_, Inr_Kleisli, inl_, Inl_Kleisli, lift_ktree_; cbn. *)
-(*   rewrite 2 bind_ret_l. *)
-(*   eapply (eutt_interp_state_iter eq eq); auto; intros. *)
-(*   rewrite 2 interp_state_bind. *)
-(*   subst. *)
-(*   eapply eutt_clo_bind; eauto. *)
-(*   intros. *)
-(*   cbn in H2; destruct H2 as [H21 H22]. *)
-(*   destruct (snd u1); rewrite <- H22. *)
-(*   - rewrite bind_ret_l, 2 interp_state_ret. *)
-(*     pstep. *)
-(*     constructor. *)
-(*     split; cbn; auto using H21. *)
-(*   - rewrite bind_ret_l, 2 interp_state_ret. pstep. constructor. *)
-(*     split; cbn; auto using H21. *)
-(* Qed. *)
-
-(* (* SAZ: These are probably too specialized. *) *)
-(* Definition state_eq {E S X} *)
-(*   : (stateT S (itree E) X) -> (stateT S (itree E) X) -> Prop := *)
-(*   fun t1 t2 => forall s, eq_itree eq (t1 s) (t2 s). *)
-
-(* Lemma interp_state_iter {E F } S (f : E ~> stateT S (itree F)) {I A} *)
-(*       (t  : I -> itree E (I + A)) *)
-(*       (t' : I -> stateT S (itree F) (I + A)) *)
-(*       (EQ_t : forall i, state_eq (State.interp_state f (t i)) (t' i)) *)
-(*   : forall i, state_eq (State.interp_state f (ITree.iter t i)) *)
-(*                   (Basics.iter t' i). *)
-(* Proof. *)
-(*   unfold Basics.iter, MonadIter_stateT0, Basics.iter, MonadIter_itree in *; cbn. *)
-(*   ginit. pcofix CIH; intros i s. *)
-(*   rewrite 2 unfold_iter; cbn. *)
-(*   rewrite !bind_bind. *)
-(*   setoid_rewrite bind_ret_l. *)
-(*   rewrite interp_state_bind. *)
-(*   guclo eqit_clo_bind; econstructor; eauto. *)
-(*   - apply EQ_t. *)
-(*   - intros [s' []] _ []; cbn. *)
-(*     + rewrite interp_state_tau. *)
-(*       gstep; constructor. *)
-(*       auto with paco. *)
-(*     + rewrite interp_state_ret; apply reflexivity. *)
-(* Qed. *)
-
-(* Lemma interp_state_iter' {E F } S (f : E ~> stateT S (itree F)) {I A} *)
-(*       (t  : I -> itree E (I + A)) *)
-(*   : forall i, state_eq (State.interp_state f (ITree.iter t i)) *)
-(*                        (Basics.iter (fun i => State.interp_state f (t i)) i). *)
-(* Proof. *)
-(*   eapply interp_state_iter. *)
-(*   intros i. *)
-(*   red. reflexivity. *)
-(* Qed. *)
-
-(* Lemma interp_state_iter'_eutt {E F S} (f: E ~> stateT S (itree F)) {I A} *)
-(*     (t : I -> itree E (I + A)) *)
-(*     (t': I -> stateT S (itree F) (I + A)) *)
-(*     (Heq: forall i s, interp_state f (t i) s ≈ (t' i) s): *)
-(*   forall i s, interp_state f (ITree.iter t i) s ≈ Basics.iter t' i s. *)
-(* Proof. *)
-(*   unfold Basics.iter, MonadIter_stateT0, Basics.iter, MonadIter_itree in *; cbn. *)
-(*   ginit. gcofix CIH; intros i s. *)
-(*   rewrite 2 unfold_iter; cbn. *)
-(*   rewrite !bind_bind. *)
-(*   setoid_rewrite bind_ret_l. *)
-(*   rewrite interp_state_bind. *)
-(*   guclo eqit_clo_bind; econstructor; eauto. *)
-(*   - apply Heq. *)
-(*   - intros [s' []] _ []; cbn. *)
-(*     + rewrite interp_state_tau. *)
-(*       gstep; constructor. *)
-(*       auto with paco. *)
-(*     + rewrite interp_state_ret; apply reflexivity. *)
-(* Qed. *)
-
-Lemma interp_state_bind {E F C D : Type -> Type} {A B S : Type}
-  `{FC : Functor C}
-  `{FD : Functor D}
-  `{C -< D}
-  (f : forall T, E T -> S -> ctree F D (S * T)%type)
-  (t : ctree E C A) (k : A -> ctree E C B)
-  (s : S) :
-  (interp_state f (t >>= k) s)
-  ~
-  (interp_state f t s >>= fun st => interp_state f (k (snd st)) (fst st)).
-Proof.
-Admitted.
-
-Unset Universe Checking.
 Lemma alloc_disjoint :
   exists m,
     @ssim Effin Effin void1 Bspec (memory * bool)%type (memory * bool)%type eq
@@ -1136,47 +793,24 @@ Lemma alloc_disjoint :
 Proof.
   eexists.
   unfold double_alloc.
-  assert ((@CTree.bind MemE void1 Z bool
-          (@CTree.trigger MemE void1 Z
-             (@subevent MemE MemE (@CategoryOps.ReSum_id (forall _ : Type, Type) IFun Id_IFun MemE) Z
-                AllocE))
-          (fun k : Z =>
-           @CTree.bind MemE void1 Z bool
-             (@CTree.trigger MemE void1 Z
-                (@subevent MemE MemE (@CategoryOps.ReSum_id (forall _ : Type, Type) IFun Id_IFun MemE)
-                   Z AllocE))
-             (fun p : Z => @ret (ctree MemE void1) (@Monad_ctree MemE void1) bool (Z.eqb k p)))) ~
-            (  vis AllocE
-    (fun k : Z =>
-     vis AllocE (fun p : Z => @ret (ctree MemE Bexec) (@Monad_ctree MemE Bexec) bool (k =? p)%Z))
-)).
-  admit.
-
-  setoid_rewrite H.
-  setoid_rewrite bind_bind.
-  rewrite interp_state_bind.
-
-
-  setoid_rewrite H.
-    ((k <- trigger AllocE;; p <- trigger AllocE;; ret (k =? p)%Z) ~ (k <- trigger AllocE;; p <- trigger AllocE;; ret (k =? p)%Z)).
-  rewrite interp_state_bind.
-  setoid_rewrite interp_state_bind.
+  repeat setoid_rewrite interp_state_bind.
   setoid_rewrite interp_state_trigger.
-  cbn.
-  setoid_rewrite bind_vis.
-
-  eapply refines_padded_refines.
-  pstep; red; cbn.
-  apply refinesF_forallL with (a:=alloc_sigma _).
-
-  cbn.
-  apply refinesF_forallL with (a:=alloc_sigma _).
-  cbn.
-
-  constructor.
+  repeat setoid_rewrite bind_bind.
+  rewrite bind_branch.
+  apply ssim_br_r with (x:=alloc_sigma _); cbn.
+  rewrite bind_ret_l.
+  rewrite bind_guard.
+  apply ssim_guard_r.
+  rewrite bind_ret_l.
+  rewrite bind_branch.
+  apply ssim_br_r with (x:=alloc_sigma _); cbn.
+  rewrite bind_ret_l.
+  rewrite bind_guard.
+  apply ssim_guard_r.
+  rewrite bind_ret_l.
+  rewrite interp_state_ret; cbn.
+  apply ssim_ret.
   reflexivity.
-  Unshelve.
-  all: constructor.
 Qed.
 
 Lemma alloc_disjoint' :
